new/golang/theory/chan.v
@@ -3,7 +3,7 @@ From New.golang.defn Require Export chan.
 From New.proof.github_com.goose_lang.goose.model.channel
   Require Import chan_init chan_au_base chan_au_send chan_au_recv.
 From iris.base_logic Require Export lib.ghost_var.
-From New.golang.theory Require Export exception loop proofmode.
+From New.golang.theory Require Export pre.
 From Perennial Require Import base.
 
 Open Scope Z_scope.
